semantics/typeSystemScript.sml
@@ -446,7 +446,7 @@ val _ = Lib.with_flag (computeLib.auto_import_definitions, false) (List.map Defn
   EVERY
     (\ (cn,ts) .  EVERY (check_freevars_ast tvs) ts /\ EVERY (check_type_names tenvT) ts)
     ctors /\
-  ~ (MEM tn (MAP (\p .  
+  ~ (MEM tn (MAP (\p .
   (case (p ) of ( (_,tn,_) ) => tn )) tds)) /\
   check_ctor_tenv tenvT tds))`;
 
@@ -674,12 +674,13 @@ type_e tenv (bind_var_list(( 0 : num)) bindings tenvE) e t)
 ==>
 type_e tenv tenvE (Letrec funs e) t)
 
-/\ (! tenv tenvE e t tdss.
+/\ (! tenv tenvE e t cg.
 (check_freevars_ast [] t /\
 check_type_names tenv.t t /\
-type_e tenv tenvE e (type_name_subst tenv.t t))
+type_e tenv tenvE e (type_name_subst tenv.t t)) /\
+type_e tenv tenvE (con_gram cg e) (Ttup [])
 ==>
-type_e tenv tenvE (Tannot e t tdss) (type_name_subst tenv.t t))
+type_e tenv tenvE (Tannot e t cg) (type_name_subst tenv.t t))
 
 /\ (! tenv tenvE e l t.
 (type_e tenv tenvE e t)
@@ -786,7 +787,7 @@ DISJOINT (LIST_TO_SET type_identities)
 check_ctor_tenv (nsAppend tenvT tenv.t) tdefs /\
 (LENGTH type_identities = LENGTH tdefs) /\
 (tenvT = alist_to_ns (MAP2
-                      (\ (tvs,tn,ctors) i . 
+                      (\ (tvs,tn,ctors) i .
                         (tn, (tvs, Tapp (MAP Tvar tvs) i)))
                       tdefs type_identities)))
 ==>
@@ -1003,4 +1004,3 @@ type_prog extra_checks decls tenv (top :: tops)
   (union_decls decls2 decls1) (extend_dec_tenv tenv2 tenv1)
   *)
 val _ = export_theory()
-
